\documentclass{article}

\usepackage[utf8]{inputenc}
\usepackage{amsmath}
\usepackage{amsfonts}
\usepackage{semantic}
\usepackage{cancel}

\input{../common}

\newcommand{\na}[0]{\ensuremath {\overset{N}{\rightarrow}}}
\newcommand{\rl}[3]{\inference{#1}{#2}\text{ #3}}
\newcommand{\bop}[0]{\ensuremath\oplus}
\newcommand{\appl}[2]{\ensuremath(#1)\ #2}
\newcommand{\st}[3][]{\ensuremath{\displaystyle\frac{#3\hfill}{#2\hfill} \text{#1}}}
\newcommand{\N}{\ensuremath \mathbb N}
\newcommand{\lam}[2]{\ensuremath{\lambda#1.#2}}
\newcommand{\inl}[0]{\ensuremath{\ inL\ }}
\newcommand{\inr}[0]{\ensuremath{\ inR\ }}
\newcommand{\case}[3]{\ensuremath{\text{case}\ #1\ \text{of}\ \left|\begin{aligned}#2\\#3\end{aligned}\right.}}
\newcommand{\Da}[0]{\ensuremath{\Downarrow}}
\usepackage{pdflscape}

\title{Assignment \#1}
\author{Diego Oniarti - 226937}
\date{}
\begin{document}

\maketitle

\section{Big step - call by name}
Write the operational semantics rules for a big-step, call-by-name reduction for ULC. Write the semantically correct ones only, but write them all

\[\begin{array}{cl}
    \st{v\Downarrow v}{} & \text{val}\\
    \\
    \st{t \bop t' \Downarrow n}{t\Downarrow n' \quad t'\Downarrow n" \quad n'\bop n" = n} & \text{bs-bop} \\
    \\
    \st{t\ t'\Downarrow v}{t\Downarrow \lam{x}{t"} \quad t"[t'/x]\Downarrow v}  & \text{bs-app} \\
    \\
    \st{\langle t_1, t_2 \rangle \Downarrow \langle v_1,v_2 \rangle}{t_1\Downarrow v_1\quad t_2\Downarrow v_2} & \text{pair} \\
    \\
    \st{t.1\Downarrow v}{t\Downarrow \langle v,v' \rangle} & \text{first-projection} \\
    \\
    \st{t.2\Downarrow v}{t\Downarrow \langle v',v \rangle} & \text{first-projection} \\
    \\
    \st{inL\ t\Downarrow inL\ v}{t\Downarrow v} & \text{inLeft} \\
    \\
    \st{inR\ t\Downarrow inR\ v}{t\Downarrow v} & \text{inRight} \\
    \\
    \st{\case{t}{\inl x_1\mapsto t_1}{\inr x_2\mapsto t_2}\Downarrow v}{t\Da \inl v' \quad t_1[v'/x_1]\Da v} & \text{pattern matching L}
    \\ \\
    \st{\case{t}{\inl x_1\mapsto t_1}{\inr x_2\mapsto t_2}\Downarrow v}{t\Da \inr v' \quad t_2[v'/x_2]\Da v} & \text{pattern matching R}
\end{array}\] 

\section{Equivalence of SOS and COS}
\subsection{if $t\to t'$ then $t\leadsto t'$}
Proof by induction on $\to$. \\
Inductive hypothesis: $\forall t_h,t_h'. if\ t_h\to t_h'\ then\ t_h\leadsto t_h'$
\subsubsection{App-2}
$t = (\lam{x}{t_1})\ t_2$ \\
$t'= (\lam{x}{t_1})\ t_2'$
\begin{align*}
    \begin{array}{rlr}
        HP1 & (\lam{x}{t_1})\ t_2 \to (\lam{x}{t_1})\ t_2' \\
        HP2 & t_2 \to t_2' \\
        TH  & (\lam{x}{t_1})\ t_2 \leadsto (\lam{x}{t_1})\ t_2' \\
        by\ IH\ with\ HP2\ w.h & t_2\leadsto t_2' & HT1 \\
        by\ inversion\ on\ HT1\ w.h & t_2 \equiv E[t_0] & HEI \\
                                    & t_2'\equiv E[t_0']  & HEI' \\
                                    & t_0 \leadsto^p t_0' & HPR \\
        by\ HEI,\ HEI'\ t.s         & (\lam{x}{t_1})\ E[t_0] \leadsto (\lam{x}{t_1})\ E[t_0'] \\
        by\ ctx\ with\ E' = (\lam{x}{t_1})\ E\ \\
        and\ HPR & (\lam{x}{t_1})\ E[t_0] \equiv E'[t_0]\leadsto E'[t_0']
    \end{array}
\end{align*}

\subsubsection{Op-1}
$t = t_1\bop t_2$ \\
$t'= t_1'\bop t_2$
\begin{align*}
    \begin{array}{rlr}
        HP1 & t_1\bop t_2 \to t_1'\bop t_2 \\
        HP2 & t_1 \to t_1' \\
        TH  & t_1\bop t_2 \leadsto t_1'\bop t_2 \\
        by\ IH\ with\ HP2\ w.h & t_1\leadsto t_1' & HT1 \\
        by\ inversion\ on\ HT1\ w.h & t_1 \equiv E[t_0] & HEI \\
                                    & t_1'\equiv E[t_0']  & HEI' \\
                                    & t_0 \leadsto^p t_0' & HPR \\
        by\ HEI,\ HEI'\ t.s         & E[t_0]\bop t_2 \leadsto E[t_0']\bop t_2 \\
        by\ ctx\ with\ E' = E\bop t_2 \\
        and\ HPR & E[t_0]\bop t_2 \equiv E'[t_0]\leadsto E'[t_0']
    \end{array}
\end{align*}

\subsubsection{Op-2}
$t = n \bop t_1$ \\
$t'= n \bop t_1'$
\begin{align*}
    \begin{array}{rlr}
        HP1 & n \bop t_1 \to n \bop t_1' \\
        HP2 & t_1 \to t_1' \\
        TH  & n \bop t_1 \leadsto n \bop t_1' \\
        by\ IH\ with\ HP2\ w.h & t_1\leadsto t_1' & HT1 \\
        by\ inversion\ on\ HT1\ w.h & t_1 \equiv E[t_0] & HEI \\
                                    & t_1'\equiv E[t_0']  & HEI' \\
                                    & t_0 \leadsto^p t_0' & HPR \\
        by\ HEI,\ HEI'\ t.s         & n \bop E[t_0] \leadsto n \bop E[t_0'] \\
        by\ ctx\ with\ E' = n \bop E \\
        and\ HPR & n\bop E[t_0]  \equiv E'[t_0]\leadsto E'[t_0']
    \end{array}
\end{align*}

\subsection{if $t\leadsto t'$ then $t\to t'$}
\paragraph{Helper lemma} $\forall t,t',E.\ if\ t\to t'\ then\ E[t]\to E[t']$ \\
Proof by induction on $E$. \\
Inductive hypothesis: $if\ t\to t'\ then\ E'[t] \to E'[t']$

\subsubsection{$E = (\lam{x}{t"})\ E'$}
\begin{align*}
    \begin{array}{rlr}
        by\ IH\ with\ HP,E'\ w.h & E'[t]\to E'[t'] & HE \\
        t.s & ((\lam{x}{t"})\ E')[t] \to ((\lam{x}{t"})\ E')[t'] \\
        by\ [\cdot]\ t.s & (\lam{x}{t"})E'[t] \to (\lam{x}{t"})E'[t'] \\
        by\ APP-1\ with\ HE & _\square
    \end{array}
\end{align*}

\subsubsection{$E = E'\bop t"$}
\begin{align*}
    \begin{array}{rlr}
        by\ IH\ with\ HP,E'\ w.h & E'[t]\to E'[t'] & HE \\
        t.s & (E\bop t")[t] \to (E\bop t")[t'] \\
        by\ [\cdot]\ t.s & E'[t] \bop t" \to E'[t']\bop t" \\
        by\ BOP-1\ with\ HE & _\square
    \end{array}
\end{align*}

\subsubsection{$E = n\bop E'$}
\begin{align*}
    \begin{array}{rlr}
        by\ IH\ with\ HP,E'\ w.h & E'[t]\to E'[t'] & HE \\
        t.s & (n\bop E')[t] \to (n\bop E')[t'] \\
        by\ [\cdot]\ t.s & n\bop E'[t] \to n\bop E'[t'] \\
        by\ BOP-1\ with\ HE & _\square
    \end{array}
\end{align*}

\section{Distinguish terms}
% ( (t -> t') -> (n -> n -> t) -> t' ) -> n
% (t -> t') -> (n -> n -> t) -> t'
\begin{multline*}
    % t\overset{def}=\lam{d:(\N\to\tau\to\tau')\to(\N\to\N\to\tau)\to\tau'\\}{d\ (\lam{m:\N}{\lam{b:\tau}{b}})\ (\lam{i:\N}{\lam{n:\N}{i}})}
    t\overset{def}=\lam{d:(\N\to\N\to\N)\to(\N\to\N\to\N)\to\N\\}{d\ (\lam{a:\N}{\lam{b:\N}{b}})\ (\lam{i:\N}{\lam{j:\N}{i}})}
\end{multline*}

\paragraph{Reduction 1}
\begin{align*}
    &\begin{array}{l @{\leadsto} c l}
        (\lam{d}{d\ (\lam{a}\lam{b}{b})\ (\lam{i}\lam{j}{i})})\ (\lam{x}\lam{y}{x\ 0\ (y\ 0\ 0)}) \\
        (\lam{x}\lam{y}{x\ 0\ (y\ 0\ 0)})\ (\lam{a}\lam{b}{b})\ (\lam{i}\lam{j}{i}) \\
        (\lam{y}{(\lam{a}\lam{b}{b})\ 0\ (y\ 0\ 0)})\ (\lam{i}\lam{j}{i}) \\
        (\lam{a}\lam{b}{b})\ 0\ ((\lam{i}\lam{j}{i})\ 0\ 0)\  \\
        (\lam{b}{b})\ ((\lam{i}\lam{j}{i})\ 0\ 0)\  \\
        (\lam{b}{b})\ ((\lam{j}{0})\ 0)\  \\
        (\lam{b}{b})\ 0 \\
    \end{array}\\
    &\quad 0
\end{align*}

\paragraph{Reduction 2}
\begin{align*}
    &\begin{array}{l @{\leadsto} c l}
        (\lam{d}{d\ (\lam{a}\lam{b}{b})\ (\lam{i}\lam{j}{i})})\ (\lam{x}\lam{y}{x\ 0\ (y\ 1\ 0)}) \\
        (\lam{x}\lam{y}{x\ 0\ (y\ 1\ 0)})\ (\lam{a}\lam{b}{b})\ (\lam{i}\lam{j}{i}) \\
        (\lam{y}{(\lam{a}\lam{b}{b})\ 0\ (y\ 1\ 0)})\ (\lam{i}\lam{j}{i}) \\
        (\lam{a}\lam{b}{b})\ 0\ ((\lam{i}\lam{j}{i})\ 1\ 0)\  \\
        (\lam{b}{b})\ ((\lam{i}\lam{j}{i})\ 1\ 0)\  \\
        (\lam{b}{b})\ ((\lam{j}{1})\ 0)\  \\
        (\lam{b}{b})\ 1 \\
    \end{array}\\
    &\quad 1
\end{align*}

% \begin{multline*}
%     t\overset{def}=\lam{d:(\N\to\tau\to\tau')\to(\N\to\N\to\tau)\\\to\tau'}{d\ (\lam{m:\N}{\lam{b:\tau}{b}})\ (\lam{i:\N}{\lam{n:\N}{i*n_1+(1-i)*n_2}})}
% \end{multline*}

\section{Safe untypable term}
\begin{equation*}
    (\lam{x}{35*12})\ (\lam{y}{1\ y})
\end{equation*}

\paragraph{typing derivation}
\begin{align*}
    \st[app]{
        \emptyset\vdash (\lam{x}{35*12})\ (\lam{y}{1\ y}): 
    }{
        \st[lam]{
            \emptyset\vdash \lam{x}{35*12}:\tau\to\N
        }{
            \st[bop]{
                x:\tau\vdash 35*12:\N
            }{
                \st[nat]{
                    x:\N\vdash 35:\N
                }{}
                \quad
                \st[nat]{
                    x:\N\vdash 12:\N
                }{}
            }
        }
        \quad
        \st[lam]{
            \emptyset\vdash \lam{y}{1\ y}: \tau'\to\tau
        }{
            \st[fail]{
                y:\tau'\vdash 1\ y: \tau
            }{}
        }
    }
\end{align*}

\paragraph{COS-SM-CBV}
\begin{align*}
    & (\lam{x}{35*12})\ (\lam{x}{1\ x}) \leadsto \\
    & 35*12 \leadsto \\
    & 420
\end{align*}

\section{Typing derivation}
\begin{equation*}
    \st[app]{
        \Gamma\left\{f:\N\to\N\right. \vdash f\ ((\lam{x}{x+2})\ 4): \N
    }{
        \st[var]{
            \Gamma \vdash f:\N\to\N
        }{
            f:\N\to\N \in \Gamma
        }
        \quad
        \st[app]{
            \Gamma\vdash (\lam{x}{x+2})\ 4: \N
        }{
            \st[lam]{
                \Gamma\vdash \lam{x}{x+2}:\N\to\N
            }{
                \st[op]{
                    \Gamma'\left\{\substack{f:\N\to\N\hfill,\\x:\N\hfill}\right.\vdash x+2:\N
                }{
                    \st[var]{
                        \Gamma'\vdash x:\N
                    }{
                        x:\N\in\Gamma'
                    }
                    \quad
                    \st[nat]{
                        \Gamma'\vdash 2:\N
                    }{
                    }
                }
            }
            \quad
            \st[nat]{
                \Gamma\vdash 4:\N
            }{}
        }
    }
\end{equation*}

\begin{equation*}
    \st[app]{
        \Gamma\left\{f:\N\to\N\right. \vdash ((\lam{x}{\lam{y}{x\ y}})\ f)\ 3:\N
    }{
        \st[app]{
            \Gamma\vdash (\lam{x}{\lam{y}{x\ y}})\ f: \N\to\N
        }{
            \st[lam]{
                \Gamma\vdash \lam{x}{\lam{y}{x\ y}}: (\N\to\N)\to\N\to\N
            }{
                \st[lam]{
                    \substack{\Gamma,\hfill\\x:\N\to\N}\vdash \lam{y}{x\ y}:\N\to\N
                }{
                    \st[app]{
                        \Gamma' \left\{ \substack{\Gamma,\hfill\\x:\N\to\N,\\y:\N\hfill} \right. \vdash x\ y:\N
                    }{
                        \st[var]{
                            \Gamma'\vdash x:\N\to\N
                        }{
                            x:\N\to\N\in\Gamma'
                        }
                        \quad
                        \st[var]{
                            \Gamma'\vdash y:\N
                        }{
                            y:\N\in\Gamma'
                        }
                    }
                }
            }
            \quad
            \st[var]{
                \Gamma\vdash f:\N\to\N
            }{
                f:\N\to\N\in\Gamma
            }
        }
        \quad
        \st[nat]{
            \Gamma\vdash 3:\N
        }{
        }
    }
\end{equation*}

\section{Encoding}
\subsection{Sequencing}
\begin{gather*}
    t ::= \cdots | t;t' \\
    t;t' \equiv (\lam{a:\tau}\lam{b:\tau'}{b})\ t\ t'
\end{gather*}
\paragraph{reductions}
\begin{align*}
    \begin{array}{r l @{\leadsto}l}
        2+4 ; 8+1 \equiv & (\lam{a}\lam{b}{b})\ (2+4)\ (8+1) \\
        (t\ \text{gets evaluated first})    & (\lam{a}\lam{b}{b})\ 6\ (8+1) \\
                                            & (\lam{b}{b})\ (8+1) \\
        (t'\ \text{gets evaluated second})  & (\lam{b}{b})\ 9 & 9
    \end{array}
\end{align*}

\paragraph{Let-in}
\begin{gather*}
    t ::= \cdots | let\ x=t\ in\ t' \\
    let\ x=t\ in\ t' \equiv (\lam{x:\tau}{t'})\ t
\end{gather*}
\paragraph{reductions}
\begin{align*}
    \begin{array}{r l @{\leadsto}l}
        let\ x=(\lam{a}\lam{b}{a*b})\ in\ x\ 11\ 13 \equiv & (\lam{x}{x\ 11\ 13})\ (\lam{a}\lam{b}{a*b}) \\
                                                           & (\lam{a}\lam{b}{a*b})\ 11\ 13 & 143 
    \end{array}
\end{align*}

\paragraph{Arrays of Length 4}
\begin{gather*}
    t ::= \cdots | [t,t,t,t] \\
    v ::= \cdots | [v,v,v,v] \\
    % [t_1,t_2,t_3,t_4] \equiv \lam{a:\tau_1\to\tau_2\to\tau_3\to\tau_4\to\tau}{a\ t_1\ t_2\ t_3\ t_4}
\end{gather*}
\begin{multline*}
    [t_1,t_2,t_3,t_4] \equiv (\lam{a:\tau_1}\lam{b:\tau_2}\lam{c:\tau_3}\\ \lam{d:\tau_4}\lam{x:\tau_1\to\tau_2\to\tau_3\to\tau_4\to\tau}{x\ a\ b\ c\ d})\ t_1\ t_2\ t_3\ t_4
\end{multline*}
\begin{equation*}
    [v_1,v_2,v_3,v_4] \equiv \lam{x:\tau_1\to\tau_2\to\tau_3\to\tau_4\to\tau}{x\ v_1\ v_2\ v_3\ v_4}
\end{equation*}
\paragraph{reductions} $[85, \lam{x}\lam{y}{x+y}, 29+44, 3]$
\begin{align*}
    &\begin{array}{l @{\leadsto}l}
        (\lam{a}\lam{b}\lam{c}\lam{d}\lam{x}{x\ a\ b\ c\ d})\ (85)\ (\lam{x}\lam{y}{x+y})\ (29+44)\ 3 \\
        (\lam{b}\lam{c}\lam{d}\lam{x}{x\ 85\ b\ c\ d})\ (\lam{x}\lam{y}{x+y})\ (29+44)\ 3 \\
        (\lam{c}\lam{d}\lam{x}{x\ 85\ (\lam{x}\lam{y}{x+y})\ c\ d})\ (29+44)\ 3 \\
        (\lam{c}\lam{d}\lam{x}{x\ 85\ (\lam{x}\lam{y}{x+y})\ c\ d})\ 73\ 3 \\
        (\lam{d}\lam{x}{x\ 85\ (\lam{x}\lam{y}{x+y})\ 73\ d})\ 3 \\
    \end{array} \\
        &\quad\lam{x}{x\ 85\ (\lam{x}\lam{y}{x+y})\ 73\ 3}
\end{align*}

\paragraph{Array field access}
\begin{gather*}
    t ::= \cdots | t.i\ (i\in0..3) \\
    t.0 \equiv t\ (\lam{a:\tau_1}\lam{b:\tau_2}\lam{c:\tau_3}\lam{d:\tau_4}{a}) \\
    t.1 \equiv t\ (\lam{a:\tau_1}\lam{b:\tau_2}\lam{c:\tau_3}\lam{d:\tau_4}{b}) \\
    t.2 \equiv t\ (\lam{a:\tau_1}\lam{b:\tau_2}\lam{c:\tau_3}\lam{d:\tau_4}{c}) \\
    t.3 \equiv t\ (\lam{a:\tau_1}\lam{b:\tau_2}\lam{c:\tau_3}\lam{d:\tau_4}{d}) \\
\end{gather*}
\paragraph{reductions $[1,1,2,3].0$}
\begin{align*}
    &\begin{array}{l @{\leadsto}l}
        ((\lam{a}\lam{b}\lam{c}\lam{d}\lam{x}{x\ a\ b\ c\ d})\ 1\ 1\ 2\ 3)\ (\lam{a}\lam{b}\lam{c}\lam{d}{a}) \\
        ((\lam{b}\lam{c}\lam{d}\lam{x}{x\ 1\ b\ c\ d})\ 1\ 2\ 3)\ (\lam{a}\lam{b}\lam{c}\lam{d}{a}) \\
        ((\lam{c}\lam{d}\lam{x}{x\ 1\ 1\ c\ d})\ 2\ 3)\ (\lam{a}\lam{b}\lam{c}\lam{d}{a}) \\
        ((\lam{d}\lam{x}{x\ 1\ 1\ 2\ d})\ 3)\ (\lam{a}\lam{b}\lam{c}\lam{d}{a}) \\
        (\lam{x}{x\ 1\ 1\ 2\ 3})\ (\lam{a}\lam{b}\lam{c}\lam{d}{a}) \\
        (\lam{a}\lam{b}\lam{c}\lam{d}{a})\ 1\ 1\ 2\ 3 \\
        (\lam{b}\lam{c}\lam{d}{1})\ 1\ 2\ 3 \\
        (\lam{c}\lam{d}{1})\ 2\ 3 \\
        (\lam{d}{1})\ 3 \\
    \end{array} \\
    & \quad 1
\end{align*}

\paragraph{Array update}
\begin{gather*}
    t ::= \cdots | t.i=t\ (i\in0..3) \\
    t.0=t' \equiv t\ ((\lam{i:\tau'}\lam{a:\tau_1}\lam{b:\tau_2}\lam{c:\tau_3}\lam{d:\tau_4}{\lam{z:\tau'\to\tau_2\to\tau_3\to\tau_4\to\tau}{z\ i\ b\ c\ d}})\ t') \\
    t.1=t' \equiv t\ ((\lam{i:\tau'}\lam{a:\tau_1}\lam{b:\tau_2}\lam{c:\tau_3}\lam{d:\tau_4}{\lam{z:\tau_1\to\tau'\to\tau_3\to\tau_4\to\tau}{z\ a\ i\ c\ d}})\ t') \\
    t.2=t' \equiv t\ ((\lam{i:\tau'}\lam{a:\tau_1}\lam{b:\tau_2}\lam{c:\tau_3}\lam{d:\tau_4}{\lam{z:\tau_1\to\tau_2\to\tau'\to\tau_4\to\tau}{z\ a\ b\ i\ d}})\ t') \\
    t.3=t' \equiv t\ ((\lam{i:\tau'}\lam{a:\tau_1}\lam{b:\tau_2}\lam{c:\tau_3}\lam{d:\tau_4}{\lam{z:\tau_1\to\tau_2\to\tau_3\to\tau'\to\tau}{z\ a\ b\ c\ i}})\ t')
\end{gather*}
\paragraph{reductions $[3,3,3,2].3=3$}
\begin{align*}
    &\begin{array}{l @{\leadsto}l}
        ((\lam{a}\lam{b}\lam{c}\lam{d}\lam{x}{x\ a\ b\ c\ d})\ 3\ 3\ 3\ 2)\ ((\lam{i}\lam{a}\lam{b}\lam{c}\lam{d}{\lam{z}{z\ a\ b\ c\ i}})\ 3) \\
        ((\lam{b}\lam{c}\lam{d}\lam{x}{x\ 3\ b\ c\ d})\ 3\ 3\ 2)\ ((\lam{i}\lam{a}\lam{b}\lam{c}\lam{d}{\lam{z}{z\ a\ b\ c\ i}})\ 3) \\
        ((\lam{c}\lam{d}\lam{x}{x\ 3\ 3\ c\ d})\ 3\ 2)\ ((\lam{i}\lam{a}\lam{b}\lam{c}\lam{d}{\lam{z}{z\ a\ b\ c\ i}})\ 3) \\
        ((\lam{d}\lam{x}{x\ 3\ 3\ 3\ d})\ 2)\ ((\lam{i}\lam{a}\lam{b}\lam{c}\lam{d}{\lam{z}{z\ a\ b\ c\ i}})\ 3) \\
        (\lam{x}{x\ 3\ 3\ 3\ 2})\ ((\lam{i}\lam{a}\lam{b}\lam{c}\lam{d}{\lam{z}{z\ a\ b\ c\ i}})\ 3) \\
        (\lam{x}{x\ 3\ 3\ 3\ 2})\ (\lam{a}\lam{b}\lam{c}\lam{d}{\lam{z}{z\ a\ b\ c\ 3}}) \\
        (\lam{a}\lam{b}\lam{c}\lam{d}{\lam{z}{z\ a\ b\ c\ 3}})\ 3\ 3\ 3\ 2 \\
        (\lam{b}\lam{c}\lam{d}{\lam{z}{z\ 3\ b\ c\ 3}})\ 3\ 3\ 2 \\
        (\lam{c}\lam{d}{\lam{z}{z\ 3\ 3\ c\ 3}})\ 3\ 2 \\
        (\lam{d}{\lam{z}{z\ 3\ 3\ 3\ 3}})\ 2 \\
    \end{array} \\
    & \quad \lam{z}{z\ 3\ 3\ 3\ 3}
\end{align*}

\end{document}
