\documentclass{article}

\usepackage[utf8]{inputenc}
\usepackage{amsmath}
\usepackage{amsfonts}
\usepackage{semantic}
\usepackage{cancel}
\usepackage{amssymb}

\input{../common}

\newcommand{\na}[0]{\ensuremath {\overset{N}{\rightarrow}}}
\newcommand{\rl}[3]{\inference{#1}{#2}\text{ #3}}
\newcommand{\bop}[0]{\ensuremath\oplus}
\newcommand{\appl}[2]{\ensuremath(#1)\ #2}
\newcommand{\st}[3][]{\ensuremath{\displaystyle\frac{#3\hfill}{#2\hfill} \text{#1}}}
\newcommand{\N}{\ensuremath \mathbb N}
\newcommand{\lam}[2]{\ensuremath{\lambda#1.#2}}
\newcommand{\inl}[0]{\ensuremath{\ inl\ }}
\newcommand{\inr}[0]{\ensuremath{\ inr\ }}
\newcommand{\case}[3]{\ensuremath{\text{case}#1\ \text{of}\ \left|\begin{aligned}#2\\#3\end{aligned}\right.}}
\newcommand{\Da}[0]{\ensuremath{\Downarrow}}
\newcommand{\while}[2]{\ensuremath{\text{while }#1\text{ do }#2\text{ end}}}
\newcommand{\for}[3]{\ensuremath{\text{for }i=#1\text{ to }#2\text{ do }#3\text{ end}}}
\newcommand{\mE}[0]{\ensuremath{\mathbb{E}}}
\newcommand{\pair}[1]{\ensuremath{\langle#1\rangle}}
\newcommand{\V}{\ensuremath{\mathcal{V}}}
\newcommand{\cE}{\ensuremath{\mathcal{E}}}
\newcommand{\cD}{\ensuremath{\mathcal{D}}}
\newcommand{\IF}[0]{\ensuremath {\text{ if }}}
\newcommand{\THEN}[0]{\ensuremath {\text{ then }}}
\newcommand{\ELSE}[0]{\ensuremath {\text{ else }}}
\newcommand{\AND}[0]{\ensuremath {\text{ and }}}
\newcommand{\OR}[0]{\ensuremath {\text{ or }}}
\newcommand{\unpack}[3]{\ensuremath{\text{unpack } #1 \text{ as }\langle #2 \rangle\text{ in }#3}}
\newcommand{\pack}[2]{\ensuremath{\text{pack } \pair{#1} \text{ as }\langle #2 \rangle}}
\usepackage{pdflscape}

\title{Assignment \#2}
\author{Diego Oniarti - 257835}
\date{}
\begin{document}

\maketitle

\section{Missing Progress Cases}
Write the proof for the progress theorem for the following cases
\begin{itemize}
    \item $t \equiv \inl t_1$
    \item $t \equiv \case{t_0}{\inl x_1 \mapsto t_1}{\inr x_2 \mapsto t_2}$
\end{itemize}

Theorem:
\[
    \text{ if } \emptyset \vdash t:\tau \text{ then either } \vdash t.VAL \text{ or } \exists t'.t\leadsto t'
\] 
Prof by induction on the typing derivation of $t$.\\
Base cases \textit{t-var} and \textit{t-nat} seen in class

\subsection{$t \equiv \inl t_1$}
\[
    \text{ if } \emptyset \vdash \inl t:\tau_1\uplus\tau_2 \text{ then either } \vdash \inl t.\text{VAL} \text{ or } \exists t'.\inl t\leadsto t'
\] 
\[
    \begin{array}{rl @{\quad} l}
                             &  \st[T-inl]{\emptyset\vdash \inl t: \tau_1\uplus\tau_2}{\emptyset\vdash t:\tau_1}  \\
        \text{t.s. either}   &   \vdash \inl t.\text{VAL} \\
        \text{or}            &   \exists t'.\inl t \leadsto t' \\
        \text{by I.H. either}&   \vdash t.\text{VAL}                 & \text{I1} \\
        \text{or}            &   \exists t".t \leadsto t"            & \text{I2} \\
    \end{array}
\]

\paragraph{Assuming I1}
$\inl t.\text{VAL}$ by I1 and definition of $\inl$. $_\square$

\paragraph{Assuming I2}
\[
    \begin{array}{rl @{\quad} l}
        \text{by inversion on I2 w.h.}   &  t \equiv \mE[t_0]         & \text{HE1}\\
                                         &  t" \equiv \mE[t_0"]        & \text{HE1'}\\
                                         &  t_0 \leadsto^p t_0"     & \text{HPR}\\
        \text{by HE1, HE1' t.s.}         &  \inl \mE[t_0] \leadsto \inl \mE[t_0"] \\
        \text{by ctx with HPR and}       &  \mE' = \inl \mE _\square \\
    \end{array}
\]

\subsection{$t \equiv \case{t_0}{\inl x_1 \mapsto t_1}{\inr x_2 \mapsto t_2}$}
\begin{multline*}
    \text{if } \underbrace{\emptyset \vdash \case{\ t_0}{\inl x_1 \mapsto t_1}{\inr x_2 \mapsto t_2}:\tau}_\text{HY} \text{ then either } \\ \cancel{ \vdash \case{t_0}{\inl x_1 \mapsto t_1}{\inr x_2 \mapsto t_2}.\text{VAL} } \\ \text{ or } \exists t'.\case{t_0}{\inl x_1 \mapsto t_1}{\inr x_2 \mapsto t_2}\leadsto t'
\end{multline*} 
\begin{align*}
    by I.H. w.h. \text{ either} & \vdash t_0.\text{VAL} & \text{I1}\\
    \text{or}                   & \exists t_0'.t_0\leadsto t_0' & \text{I2}
\end{align*}

\paragraph{Assuming I1}
\begin{equation*}
    \text{by typing definition of $case$ and HY}\begin{array}{r@{\quad}l} 
        \text{either} & t_0 \equiv \inl t_0^l \\
        \text{or}     & t_0 \equiv \inr t_0^r
    \end{array}
\end{equation*}
\begin{itemize}
    \item $t_0\equiv\inl t_0^l$ \\
            by COS rule for $case$: $\case{\inl t_0^l}{\inl x_1 \mapsto t_1}{\inr x_2 \mapsto t_2} \leadsto^p t_1[t_0^l/x_1]_\square$ \\

    \item $t_0\equiv\inr t_0^r$ \\
        by COS rule for case: $\case{\inr t_0^r}{\inl x_1 \mapsto t_1}{\inr x_2 \mapsto t_2} \leadsto^p t_2[t_0^r/x_2]_\square$
\end{itemize}
\paragraph{Assuming I2}
\[
    \begin{array}{rl @{\quad} l}
        \text{by inversion on I2 w.h.}   &  t_0  \equiv \mE[t_0^z]         & \text{HE1}\\
                                         &  t_0' \equiv \mE[t_0'^z]        & \text{HE1'}\\
                                         &  t_0^z \leadsto^p t_0'^z     & \text{HPR}\\
        \text{by HE1, HE1' t.s.}         &  \case{\ \mE[t_0^z]}{\inl x_1 \mapsto t_1}{\inr x_2 \mapsto t_2} \leadsto \case{\ \mE[t_0'^z]}{\inl x_1 \mapsto t_1}{\inr x_2 \mapsto t_2} \\
        \text{by ctx with HPR and}       &  \mE' = \case{\ \mE}{\inl x_1 \mapsto t_1}{\inr x_2 \mapsto t_2} _\square \\
    \end{array}
\]


\section{Missing Compatibility Lemmas}
Write the proof for these compatibility lemmas:
\begin{itemize}
    \item Pairs \\
        Assuming: \begin{itemize}
            \item $\Gamma \vDash t_1:\tau_1$ (HP1)
            \item $\Gamma \vDash t_2:\tau_2$ (HP2)
        \end{itemize}
        Prove: \begin{itemize}
            \item $\Gamma \vDash \langle t_1,t_2 \rangle : \tau_1\times\tau_2$
        \end{itemize}
        \begin{align*}
            \text{by def. ST take} &\ \gamma \in G[\tau] \\
            \text{t.s.} &\ \pair{t_1,t_2}\gamma\in\cE[\tau_1,\tau_2] \\
            \text{by def. $\cE$ t.s.} &\ \exists v.\pair{t_1,t_2}\gamma\leadsto^{*}v\AND v\in\V[\tau_1\times\tau_2] \\
            \text{by HP1 w.h.} &\ t_1\in\cE[\tau_1] & (A1) \\
            \text{by A1 and def. $\cE$ w.h.} &\ \exists v_1.t_1 \leadsto^{*}v_1\AND v_1\in\V[\tau_1] & (A2) \\
            \text{by HP2 w.h.} &\ t_2\in\cE[\tau_2] & (B1) \\
            \text{by B1 and def. $\cE$ w.h.} &\ \exists v_2.t_2 \leadsto^{*}v_2\AND v_2\in\V[\tau_2] & (B2) \\
            \text{by A2,B2 w.h.} &\ \pair{t_1,t_2}\gamma \leadsto^{*}\pair{v_1,v_2} & (C1) \\
            \text{by C1 and def. $\V[\tau_1\times\tau_2]$ w.h.} &\ v\equiv\pair{v_1,v_2}\in\V[\tau_1\times\tau_2]_\square
        \end{align*}

    \item Projection \\
        Assuming: \begin{itemize}
            \item $\Gamma \vDash t:\tau_1\times\tau_2$ (HP)
        \end{itemize}
        Prove: \begin{itemize}
            \item $\Gamma \vDash t.1:\tau_1$
        \end{itemize}
        \begin{align*}
            \text{by def. ST take} &\ \gamma\in G[\tau] \\
            \text{t.s.} &\ t.1\gamma \in \cE[\tau_1] \\
            \text{by def $\cE$ t.s.} &\ \exists v_1.\ t.1\leadsto^{*} v_1\AND v_1\in\V[\tau_1] & (B1) \\
            \text{by HP and def. ST w.h.} &\ \exists v.\ t\leadsto^{*} v\AND v\in\V[\tau_1\times\tau_2] & (A1) \\
            \text{by A1 and def. $\V_\times$ w.h.} &\ v\equiv \pair{v_1',v_2'} \AND v_1' \in \V[\tau_1] & (A2) \\
            \text{by A1,A2 with} &\ v_1'=v_1\ B1\ holds_\square
        \end{align*}

    \item Unpack \\
        Assuming: \begin{itemize}
            \item $\Delta \vdash \tau'$ (HP1)
            \item $\Delta,\Gamma \vDash t:\exists\alpha.\tau$ (HP2)
            \item $\Delta;\alpha,\Gamma;x : \tau\vDash t':\tau'$ (HP3)
        \end{itemize}
        Prove: \begin{itemize}
            \item $\Delta,\Gamma\vDash \unpack{t}{\alpha,x}{t'} \tau'$
        \end{itemize}
        \begin{align*}
            \text{by  def. ST take} &\ \delta\in\cD[\Delta],\gamma\in G[\Gamma]^\delta \\
            \text{t.s.} &\ (\unpack{t}{\alpha,x}{t'})^\delta\gamma\in\cE[\tau']^\delta & (TY) \\
            \text{by def. $\cE$ t.s.} &\ \exists v.(\unpack{t}{\alpha,x}{t'})^\delta\gamma\in\cE[\tau']^\delta \leadsto^{*} v \\
            \text{and}                &\ v\in\V[\tau']^\delta \\
        \end{align*}
        From this point on the proof is trivial and left to the reader
\end{itemize}

\section{Adding Cycles}
Add \texttt{for} and \texttt{while} constructs to STLC. Add their syntax, their typing and their operational
semantics in COS.

\subsection{while}
\begin{align*}
    t = \cdots |& \while{t}{t} \\
    v = \cdots |& \Xi \\
    \tau = \cdots |& \xi \\
    \mE = \cdots |& \while{\mE}{t} \\
                 %|& \while{true}{\mE}
\end{align*}
\begin{gather*}
    \st[t-while]{\Gamma\vdash \while{t_0}{t_1}: \xi }{\Gamma\vdash t_0:bool \quad \Gamma\vdash t_1:\tau} \\
    \\
    \st[c-whileT]{\while{true}{t} \leadsto^p t;\while{true}{t} }{} \\
    \\
    \st[c-whileF]{\while{false}{t} \leadsto^p \Xi }{}
\end{gather*}

\subsection{for}
\begin{align*}
    t = \cdots |& \for{t}{t}{t} \\
    v = \cdots |& \Xi \\
    \tau = \cdots |& \xi \\
    \mE = \cdots  |& \for{\mE}{t}{t} \\
                  |& \for{n}{\mE}{t} \\
                  %|& \for{n}{n}{\mE} \\
\end{align*}
\begin{gather*}
    \st[t-for]{\Gamma\vdash \for{t_0}{t_1}{t_2}: \xi }{\Gamma\vdash t_0:\N \quad \Gamma\vdash t_1:\N \quad \Gamma,i:\N\vdash t_2:\tau} \\
    \\
    \st[c-for1]{
        \for{n_1}{n_2}{t} \leadsto^p t[n_1/i];\for{n_1'}{n_2}{t}
    }{
        n_1<n_2
        \quad
        n_1' = n_1+1
    } \\
    \\
    \st[c-for2]{
        \for{n_1}{n_2}{t} \leadsto^p \Xi
    }{
        n_1\geq n_2
    } \\
\end{gather*}


\end{document}
